cogent/isa/TypeTrackingTyping2.thy
@@ -1,0 +1,632 @@
+(*
+ * Copyright 2016, NICTA
+ *
+ * This software may be distributed and modified according to the terms of
+ * the GNU General Public License version 2. Note that NO WARRANTY is provided.
+ * See "LICENSE_GPLv2.txt" for details.
+ *
+ * @TAG(NICTA_GPL)
+ *)
+
+theory TypeTrackingTyping2 imports
+  Cogent
+begin
+
+datatype type_split_kind = TSK_L | TSK_R | TSK_S | TSK_NS | TSK_NONE
+
+datatype ttctx = CtxSplit "type_split_kind list" ttctx ttctx | CtxSplitTriv ttctx ttctx | CtxLeaf
+
+fun apply_tsk :: "type_split_kind \<Rightarrow> type option \<Rightarrow> type option \<times> type option"
+where
+    "apply_tsk TSK_NONE None     = (None, None)"
+  | "apply_tsk TSK_L    (Some t) = (Some t, None)"
+  | "apply_tsk TSK_R    (Some t) = (None, Some t)"
+  | "apply_tsk TSK_S    (Some t) = (Some t, Some t)"
+  | "apply_tsk TSK_NS   (Some t) = (Some (bang t), Some t)"
+  | "apply_tsk TSK_NONE (Some _) = undefined"
+  | "apply_tsk _        None     = undefined"
+
+definition apply_tsks :: "type_split_kind list \<Rightarrow> ctx \<Rightarrow> ctx \<times> ctx" where
+  "apply_tsks sps \<Gamma> = unzip (List.map2 apply_tsk sps \<Gamma>)"
+
+fun verify_tsk :: "kind env \<Rightarrow> type_split_kind \<Rightarrow> type option \<Rightarrow> bool"
+where
+    "verify_tsk K TSK_NONE None     = True"
+  | "verify_tsk K TSK_L    (Some t) = (\<exists>k. K \<turnstile> t :\<kappa> k)"
+  | "verify_tsk K TSK_R    (Some t) = (\<exists>k. K \<turnstile> t :\<kappa> k)"
+  | "verify_tsk K TSK_S    (Some t) = (\<exists>k. K \<turnstile> t :\<kappa> k \<and> S \<in> k)"
+  | "verify_tsk K TSK_NS   (Some t) = (\<exists>k. K \<turnstile> t :\<kappa> k)"
+  | "verify_tsk _ TSK_NONE (Some _) = False"
+  | "verify_tsk _ _        None     = False"
+
+definition verify_tsks :: "kind env \<Rightarrow> type_split_kind list \<Rightarrow> ctx \<Rightarrow> bool" where
+  "verify_tsks K = list_all2 (verify_tsk K)"
+
+inductive syntactic_subtype :: "type \<Rightarrow> type \<Rightarrow> bool" where
+  syn_subty_refl: "syntactic_subtype \<tau> \<tau>"
+| syn_subty_tfun_in: "syntactic_subtype \<tau> \<tau>1 \<Longrightarrow> syntactic_subtype \<tau> (TFun \<tau>1 \<tau>2)"
+| syn_subty_tfun_out: "syntactic_subtype \<tau> \<tau>2 \<Longrightarrow> syntactic_subtype \<tau> (TFun \<tau>1 \<tau>2)"
+| syn_subty_tcon: "\<lbrakk> t \<in> set \<tau>s ; syntactic_subtype \<tau> t \<rbrakk> \<Longrightarrow> syntactic_subtype \<tau> (TCon n \<tau>s s)"
+| syn_subty_tsum: "\<lbrakk> t \<in> set \<tau>s ; syntactic_subtype \<tau> (snd t) \<rbrakk> \<Longrightarrow> syntactic_subtype \<tau> (TSum \<tau>s)"
+| syn_subty_tprod_l: "syntactic_subtype \<tau> \<tau>1 \<Longrightarrow> syntactic_subtype \<tau> (TProduct \<tau>1 \<tau>2)"
+| syn_subty_tprod_r: "syntactic_subtype \<tau> \<tau>2 \<Longrightarrow> syntactic_subtype \<tau> (TProduct \<tau>1 \<tau>2)"
+| syn_subty_trec: "\<lbrakk> t \<in> set \<tau>s ; syntactic_subtype \<tau> (fst t) \<rbrakk> \<Longrightarrow> syntactic_subtype \<tau> (TRecord \<tau>s s)"
+
+fun syntactic_subtypes :: "type \<Rightarrow> type set" where
+  "syntactic_subtypes (TVar i)       = {TVar i}"
+| "syntactic_subtypes (TVarBang i)   = {TVarBang i}"
+| "syntactic_subtypes (TCon n ts s)  = {TCon n ts s} \<union> (\<Union>(syntactic_subtypes ` set ts))"
+| "syntactic_subtypes (TFun a b)     = {TFun a b} \<union> syntactic_subtypes a \<union> syntactic_subtypes b"
+| "syntactic_subtypes (TPrim p)      = {TPrim p}"
+| "syntactic_subtypes (TSum ts)      = {TSum ts} \<union> (\<Union>((syntactic_subtypes \<circ> snd) ` set ts))"
+| "syntactic_subtypes (TProduct a b) = {TProduct a b} \<union> syntactic_subtypes a \<union> syntactic_subtypes b"
+| "syntactic_subtypes (TRecord ts s) = {TRecord ts s} \<union> (\<Union>((syntactic_subtypes \<circ> fst) ` set ts))"
+| "syntactic_subtypes (TUnit)        = {TUnit}"
+
+lemma "t \<in> syntactic_subtypes \<tau> \<Longrightarrow> syntactic_subtype t \<tau>"
+  by (induct \<tau> arbitrary: t rule: syntactic_subtypes.induct)
+    (force intro: syntactic_subtype.intros)+
+
+lemma syntactic_subtypes_refl: "\<tau> \<in> syntactic_subtypes \<tau>"
+  by (induct \<tau>) simp+
+
+lemma "syntactic_subtype t \<tau> \<Longrightarrow> t \<in> syntactic_subtypes \<tau>"
+  by (induct rule: syntactic_subtype.inducts)
+    (fastforce simp add: syntactic_subtypes_refl)+
+
+
+section {* Fast Kinding *}
+
+(* droppable+sharable, escapable *)
+type_synonym kind' = "bool \<times> bool"
+
+definition kind_isD :: "kind' \<Rightarrow> bool" where
+  "kind_isD \<equiv> fst"
+
+definition kind_isS :: "kind' \<Rightarrow> bool" where
+  "kind_isS \<equiv> fst"
+
+definition kind_isE :: "kind' \<Rightarrow> bool" where
+  "kind_isE \<equiv> snd"
+
+fun kind'_inter :: "kind' \<Rightarrow> kind' \<Rightarrow> kind'" where
+  "kind'_inter (ds1, e1) (ds2, e2) = (ds1 \<and> ds2, e1 \<and> e2)"
+
+fun sigil_kind' :: "sigil \<Rightarrow> kind'" where
+  "sigil_kind' ReadOnly = (True, False)"
+| "sigil_kind' Writable = (False, True)"
+| "sigil_kind' Unboxed  = (True, True)"
+
+fun wellformed' :: "nat \<Rightarrow> type \<Rightarrow> bool" where
+  "wellformed' n (TVar i)       = (i < n)"
+| "wellformed' n (TVarBang i)   = (i < n)"
+| "wellformed' n (TCon _ ts s)  = foldl (\<and>) True (map (wellformed' n) ts)"
+| "wellformed' n (TFun t u)     = (wellformed' n t \<and> wellformed' n u)"
+| "wellformed' n (TPrim p)      = True"
+| "wellformed' n (TSum ts)      = foldl (\<and>) True (map (wellformed' n \<circ> snd) ts)"
+| "wellformed' n (TProduct t u) = (wellformed' n t \<and> wellformed' n u)"
+| "wellformed' n (TRecord ts s) = foldl (\<and>) True (map (wellformed' n \<circ> fst) ts)"
+| "wellformed' n (TUnit)        = True"
+
+fun kinding' :: "kind' env \<Rightarrow> type \<Rightarrow> kind'" where
+  "kinding' K (TVar i)       = (K ! i)"
+| "kinding' K (TVarBang i)   = (True, snd (K ! i))"
+| "kinding' K (TCon _ ts s)  = kind'_inter (foldl kind'_inter (True, True) (map (kinding' K) ts)) (sigil_kind' s)"
+| "kinding' K (TFun t u)     = kind'_inter (kinding' K t) (kinding' K u)"
+| "kinding' K (TPrim p)      = (True, True)"
+| "kinding' K (TSum ts)      = foldl kind'_inter (True, True) (map (kinding' K \<circ> snd) ts)"
+| "kinding' K (TProduct t u) = kind'_inter (kinding' K t) (kinding' K u)"
+| "kinding' K (TRecord ts s) = foldl kind'_inter (True, True) (map (\<lambda>(t,b). if b then (True,True) else (kinding' K t)) ts)"
+| "kinding' K (TUnit)        = (True, True)"
+
+
+lemma foldl_kind'_inter_short_circuit:
+  "foldl kind'_inter (False, False) ts = (False, False)"
+  by (induct ts) (clarsimp+)
+
+lemma foldl_map_evalsimps:
+  "foldl f init (map g []) = init"
+  "foldl f init (map g (x # xs)) = foldl f (f init (g x)) (map g xs)"
+  by clarsimp+
+
+lemmas kinding'_simps =
+  kinding'.simps kind'_inter.simps foldl_map_evalsimps sigil_kind'.simps HOL.simp_thms(21-25)
+  fst_conv snd_conv Product_Type.split if_True if_False
+
+section {* ttyping *}
+
+inductive ttyping :: "('f \<Rightarrow> poly_type) \<Rightarrow> kind env \<Rightarrow> ctx \<Rightarrow> ttctx \<Rightarrow> 'f expr \<Rightarrow> type \<Rightarrow> bool" 
+          ("_, _, _, _ T\<turnstile> _ : _" [55,0,0,0,55] 60)
+and ttyping_all :: "('f \<Rightarrow> poly_type) \<Rightarrow> kind env \<Rightarrow> ctx \<Rightarrow> ttctx \<Rightarrow> 'f expr list \<Rightarrow> type list \<Rightarrow> bool" 
+          ("_, _, _, _ T\<turnstile>* _ : _" [55,0,0,0,55] 60)
+where
+
+  typing_var    : "\<lbrakk> K \<turnstile> \<Gamma> \<leadsto>w singleton (length \<Gamma>) i t (* TODO *)
+                   ; i < length \<Gamma>
+                   \<rbrakk> \<Longrightarrow> \<Xi>, K, \<Gamma>, CtxLeaf T\<turnstile> Var i : t"
+
+| typing_app    : "\<lbrakk> verify_tsks K sps \<Gamma>
+                   ; apply_tsks sps \<Gamma> = (\<Gamma>1, \<Gamma>2)
+                   ; \<Xi>, K, \<Gamma>1, t1 T\<turnstile> a : TFun x y
+                   ; \<Xi>, K, \<Gamma>2, t2 T\<turnstile> b : x 
+                   \<rbrakk> \<Longrightarrow> \<Xi>, K, \<Gamma>, CtxSplit sps T1 T2 T\<turnstile> App a b : y"
+
+| typing_con    : "\<lbrakk> \<Xi>, K, \<Gamma>, T T\<turnstile> x : t
+                   ; (tag,t) \<in> set ts
+                   ; K \<turnstile>* (map snd ts) wellformed
+                   ; distinct (map fst ts)
+                   \<rbrakk> \<Longrightarrow> \<Xi>, K, \<Gamma>, T T\<turnstile> Con ts tag x : TSum ts"
+
+| ttyping_split  : "\<lbrakk> verify_tsks K sps \<Gamma>
+                   ; apply_tsks sps \<Gamma> = (\<Gamma>1, \<Gamma>2')
+                   ; \<Xi>, K, \<Gamma>1, T1 T\<turnstile> x : TProduct t u
+                   ; \<Gamma>2 = [Some t, Some u] @ \<Gamma>2'
+                   ; \<Xi>, K, \<Gamma>2, T2 T\<turnstile> y : t'
+                   \<rbrakk> \<Longrightarrow> \<Xi>, K, \<Gamma>, CtxSplit sps T1 T2 T\<turnstile> Split x y : t'"
+
+| ttyping_let    : "\<lbrakk> verify_tsks K sps \<Gamma>
+                   ; apply_tsks sps \<Gamma> = (\<Gamma>1, \<Gamma>2')
+                   ; \<Xi>, K, \<Gamma>1, T1 T\<turnstile> x : t
+                   ; \<Gamma>2 = [Some t] @ \<Gamma>2'
+                   ; \<Xi>, K, \<Gamma>2, T2 T\<turnstile> y : u
+                   \<rbrakk> \<Longrightarrow> \<Xi>, K, \<Gamma>, CtxSplit sps T1 T2 T\<turnstile> Let x y : u"
+
+| ttyping_letb   : "\<lbrakk> verify_tsks K sps \<Gamma>
+                   ; apply_tsks sps \<Gamma> = (\<Gamma>1, \<Gamma>2')
+                   ; \<Xi>, K, \<Gamma>1, T1 T\<turnstile> x : t
+                   ; \<Gamma>2 = [Some t] @ \<Gamma>2'
+                   ; \<Xi>, K, \<Gamma>2, T2 T\<turnstile> y : u
+                   ; K \<turnstile> t :\<kappa> k
+                   ; E \<in> k
+                   \<rbrakk> \<Longrightarrow> \<Xi>, K, \<Gamma>, CtxSplit sps T1 T2 T\<turnstile> LetBang is x y : u"
+
+| ttyping_case   : "\<lbrakk> verify_tsks K sps \<Gamma>
+                   ; apply_tsks sps \<Gamma> = (\<Gamma>1, \<Gamma>2)
+                   ; (tag, t) \<in> set ts
+                   ; \<Xi>, K, \<Gamma>1, T1 T\<turnstile> x : TSum ts
+                   ; \<Gamma>21 = [Some t] @ \<Gamma>2
+                   ; \<Gamma>22 = [Some (TSum (filter (\<lambda> x. fst x \<noteq> tag) ts))] @ \<Gamma>2
+                   ; \<Xi>, K, \<Gamma>21, T21 T\<turnstile> a : u
+                   ; \<Xi>, K, \<Gamma>22, T22 T\<turnstile> b : u
+                   \<rbrakk> \<Longrightarrow> \<Xi>, K, \<Gamma>, CtxSplit sps T1 (CtxSplitTriv T21 T22) T\<turnstile> Case x tag a b : u" 
+
+| ttyping_if     : "\<lbrakk> verify_tsks K sps \<Gamma>
+                   ; apply_tsks sps \<Gamma> = (\<Gamma>1, \<Gamma>2)
+                   ; \<Xi>, K, \<Gamma>1, T1 T\<turnstile> x : TPrim Bool
+                   ; \<Xi>, K, \<Gamma>2, T21 T\<turnstile> a : t
+                   ; \<Xi>, K, \<Gamma>2, T22 T\<turnstile> b : t
+                   \<rbrakk> \<Longrightarrow> \<Xi>, K, \<Gamma>, CtxSplit sps T1 (CtxSplitTriv T21 T22) T\<turnstile> If x a b : t"
+
+| ttyping_take   : "\<lbrakk> verify_tsks K sps \<Gamma>
+                   ; apply_tsks sps \<Gamma> = (\<Gamma>1, \<Gamma>2')
+                   ; s \<noteq> ReadOnly
+                   ; f < length ts
+                   ; ts ! f = (t, False)
+                   ; K \<turnstile> t :\<kappa> k
+                   ; S \<in> k \<or> taken
+                   ; \<Xi>, K, \<Gamma>1, T1 T\<turnstile> e : TRecord ts s
+                   ; \<Gamma>2 = [Some t, Some (TRecord (ts [f := (t, taken)]) s)] @ \<Gamma>2'
+                   ; \<Xi>, K, \<Gamma>2, T2 T\<turnstile> e' : u
+                   \<rbrakk> \<Longrightarrow> \<Xi>, K, \<Gamma>, CtxSplit sps T1 T2 T\<turnstile> Take e f e' : u"
+
+| typing_put    : "\<lbrakk> verify_tsks K sps \<Gamma>
+                   ; apply_tsks sps \<Gamma> = (\<Gamma>1, \<Gamma>2')
+                   ; \<Xi>, K, \<Gamma>1, T1 T\<turnstile> e : TRecord ts s
+                   ; ts' = (ts [f := (t,False)])
+                   ; s \<noteq> ReadOnly
+                   ; f < length ts
+                   ; ts ! f = (t, taken)
+                   ; K \<turnstile> t :\<kappa> k
+                   ; D \<in> k \<or> taken
+                   ; \<Xi>, K, \<Gamma>2, T2 T\<turnstile> e' : t
+                   \<rbrakk> \<Longrightarrow> \<Xi>, K, \<Gamma>, CtxSplit sps T1 T2 T\<turnstile> Put e f e' : TRecord ts' s"
+
+| typing_all_empty : "\<Gamma> = empty n \<Longrightarrow> \<Xi>, K, \<Gamma>, CtxLeaf T\<turnstile>* [] : []"
+
+| typing_all_cons  : "\<lbrakk> verify_tsks K sps \<Gamma>
+                      ; apply_tsks sps \<Gamma> = (\<Gamma>1, \<Gamma>2)
+                      ; \<Xi>, K, \<Gamma>1, T1 T\<turnstile>  e  : t
+                      ; \<Xi>, K, \<Gamma>2, T2 T\<turnstile>* es : ts
+                      \<rbrakk> \<Longrightarrow> \<Xi>, K, \<Gamma>, CtxSplit sps T1 T2 T\<turnstile>* e # es : t # ts"
+
+
+section {* Wellformed/Kinding as a function *}
+
+fun wellformed_fn :: "nat \<Rightarrow> type \<Rightarrow> bool" where
+  "wellformed_fn n (TVar i) = (i < n)"
+| "wellformed_fn n (TVarBang i) = (i < n)"
+| "wellformed_fn n (TCon _ ts _) = list_all (\<lambda>x. wellformed_fn n x) ts"
+| "wellformed_fn n (TFun t1 t2) = (wellformed_fn n t1 \<and> wellformed_fn n t2)"
+| "wellformed_fn n (TPrim _) = True"
+| "wellformed_fn n (TSum ts) = (distinct (map fst ts) \<and> (list_all (\<lambda>x. wellformed_fn n (snd x)) ts))"
+| "wellformed_fn n (TProduct t1 t2) = (wellformed_fn n t1 \<and> wellformed_fn n t2)"
+| "wellformed_fn n (TRecord ts _) = (list_all (\<lambda>x. wellformed_fn n (fst x)) ts)"
+| "wellformed_fn n TUnit = True"
+
+definition ctx_wellformed_fn where
+  "ctx_wellformed_fn n \<Gamma> \<equiv> list_all (\<lambda>t. \<forall>t'. t = Some t' \<longrightarrow> wellformed_fn n t') \<Gamma>"
+
+lemmas ctx_wellformed_fn_nil =
+  list_all_nil[where P=\<open>\<lambda>t. \<forall>t'. t = Some t' \<longrightarrow> wellformed_fn n t'\<close> for n, simplified ctx_wellformed_fn_def[symmetric]]
+lemmas ctx_wellformed_fn_cons =
+ list_all_cons[where P=\<open>\<lambda>t. \<forall>t'. t = Some t' \<longrightarrow> wellformed_fn n t'\<close> for n, simplified ctx_wellformed_fn_def[symmetric]]
+
+lemmas ctx_wellformed_fn_Cons =
+ list.pred_inject(2)[where P=\<open>\<lambda>t. \<forall>t'. t = Some t' \<longrightarrow> wellformed_fn n t'\<close> for n, simplified ctx_wellformed_fn_def[symmetric]]
+
+fun kinding_fn :: "kind env \<Rightarrow> type \<Rightarrow> kind" where
+  "kinding_fn K (TVar i)         = K ! i"
+| "kinding_fn K (TVarBang i)     = {D,S}"
+| "kinding_fn K (TCon n ts s)    = Inter (set (map (kinding_fn K) ts)) \<inter> (sigil_kind s)"
+| "kinding_fn K (TFun ta tb)     = UNIV"
+| "kinding_fn K (TPrim p)        = UNIV"
+| "kinding_fn K (TSum ts)        = Inter (set (map (kinding_fn K \<circ> snd) ts))"
+| "kinding_fn K (TProduct ta tb) = kinding_fn K ta \<inter> kinding_fn K tb"
+| "kinding_fn K (TRecord ts s)   = Inter (set (map (\<lambda>(t,b). case b of False \<Rightarrow> kinding_fn K t | True \<Rightarrow> UNIV) ts)) \<inter> (sigil_kind s)"
+| "kinding_fn K TUnit            = UNIV"
+
+lemma kinding_imp_wellformedfn:
+  "K \<turnstile> t :\<kappa> k \<Longrightarrow> wellformed_fn (length K) t"
+  "K \<turnstile>* ts :\<kappa> k \<Longrightarrow> list_all (wellformed_fn (length K)) ts"
+  "K \<turnstile>* tsr :\<kappa>r k \<Longrightarrow> list_all (wellformed_fn (length K) \<circ> fst) tsr"
+  by (induct rule: kinding_kinding_all_kinding_record.inducts) (simp add: list_all_iff)+
+
+lemma kinding_imp_kinding_fn:
+  "K \<turnstile> t :\<kappa> k \<Longrightarrow> k \<subseteq> kinding_fn K t"
+  "K \<turnstile>* ts :\<kappa> k \<Longrightarrow> k \<subseteq> Inter (set (map (kinding_fn K) ts))"
+  "K \<turnstile>* tsr :\<kappa>r k \<Longrightarrow> k \<subseteq> Inter (set (map (\<lambda>(t,b). case b of False \<Rightarrow> kinding_fn K t | True \<Rightarrow> UNIV) tsr))"
+  by (induct rule: kinding_kinding_all_kinding_record.inducts) (simp add: list_all_iff)+
+
+lemma wellformedfn_and_kindingfn_imp_kinding:
+  "\<lbrakk> wellformed_fn (length K) t; k \<subseteq> kinding_fn K t \<rbrakk> \<Longrightarrow> K \<turnstile> t :\<kappa> k"
+proof (induct t arbitrary: k)
+  case TCon then show ?case
+    by (fastforce intro!: kinding_kinding_all_kinding_record.intros simp add: kinding_all_set INT_subset_iff list.pred_set)
+next
+  case TSum then show ?case
+    by (fastforce intro!: kinding_kinding_all_kinding_record.intros simp add: kinding_all_set INT_subset_iff list.pred_set)
+next
+  case (TRecord x1a x2a)
+  then show ?case
+    apply (auto intro!: kinding_kinding_all_kinding_record.intros simp add: kinding_record_set kinding_all_set INT_subset_iff list.pred_set)
+     apply (metis fst_conv order_refl)
+    apply fastforce
+    done
+qed (auto intro!: kinding_kinding_all_kinding_record.intros)
+
+lemma kinding_iff_wellformedfn_and_kindingfn:
+  "K \<turnstile> t :\<kappa> k \<longleftrightarrow> wellformed_fn (length K) t \<and> k \<subseteq> kinding_fn K t"
+  by (meson
+      kinding_imp_kinding_fn kinding_imp_wellformedfn wellformedfn_and_kindingfn_imp_kinding)
+
+lemma wellformed_iff_wellformedfn:
+  "K \<turnstile> t wellformed \<longleftrightarrow> wellformed_fn (length K) t"
+  by (force simp add: kinding_iff_wellformedfn_and_kindingfn)
+
+lemma wellformed_all_iff_wellformedfn_all:
+  "K \<turnstile>* ts wellformed \<longleftrightarrow> list_all (wellformed_fn (length K)) ts"
+  by (clarsimp
+      simp del: type_wellformed_all_def type_wellformed_def
+      simp add: type_wellformed_all_subkind_weaken wellformed_iff_wellformedfn)
+
+lemma wellformed_kindingfn_always_kinding:
+  "\<lbrakk> wellformed_fn (length K) t; k = kinding_fn K t \<rbrakk> \<Longrightarrow> K \<turnstile> t :\<kappa> k"
+  by (clarsimp simp add: kinding_iff_wellformedfn_and_kindingfn)
+
+lemma wellformedfn_preserves_bang:
+  assumes "wellformed_fn n t"
+  shows "wellformed_fn n (bang t)"
+  using assms
+  by (induct t arbitrary: n) (force simp add: list_all_iff split: prod.split)+
+
+lemma wellformedfn_preserves_instantiate:
+  assumes
+    "list_all (wellformed_fn n') \<delta>"
+    "length \<delta> = n"
+    "wellformed_fn n t"
+  shows "wellformed_fn n' (instantiate \<delta> t)"
+  using assms
+  by (induct t arbitrary: n n') (force simp add: list_all_iff intro: wellformedfn_preserves_bang)+
+
+lemma split_preserves_wellformed:
+  assumes
+    "K \<turnstile> \<Gamma> \<leadsto> \<Gamma>1 | \<Gamma>2"
+    "ctx_wellformed_fn (length K) \<Gamma>"
+  shows
+    "ctx_wellformed_fn (length K) \<Gamma>1"
+    "ctx_wellformed_fn (length K) \<Gamma>2"
+using assms
+  by (induct rule: split_inducts) (fastforce elim: split_comp.cases simp add: ctx_wellformed_fn_def)+
+
+lemma split_bang_preserves_wellformed:
+  assumes
+    "K , is \<turnstile> \<Gamma> \<leadsto>b \<Gamma>1 | \<Gamma>2"
+    "ctx_wellformed_fn (length K) \<Gamma>"
+  shows
+    "ctx_wellformed_fn (length K) \<Gamma>1"
+    "ctx_wellformed_fn (length K) \<Gamma>2"
+using assms
+  by (induct rule: split_bang.inducts)
+    (force intro: wellformedfn_preserves_bang simp: split_comp.simps split_bang_comp.simps ctx_wellformed_fn_def)+
+
+
+section {* Minimal Wellformed typing *}
+
+inductive typing2 :: "('f \<Rightarrow> poly_type) \<Rightarrow> kind env \<Rightarrow> ctx \<Rightarrow> 'f expr \<Rightarrow> type \<Rightarrow> bool" 
+          ("_, _, _ \<turnstile>2 _ : _" [55,0,0,0,55] 60)
+      and typing2_all :: "('f \<Rightarrow> poly_type) \<Rightarrow> kind env \<Rightarrow> ctx \<Rightarrow> 'f expr list \<Rightarrow> type list \<Rightarrow> bool"
+          ("_, _, _ \<turnstile>2* _ : _" [55,0,0,0,55] 60) where
+
+  typing_var    : "\<lbrakk> K \<turnstile> \<Gamma> \<leadsto>w singleton (length \<Gamma>) i t 
+                   ; i < length \<Gamma>
+                   \<rbrakk> \<Longrightarrow> \<Xi>, K, \<Gamma> \<turnstile>2 Var i : t"
+
+| typing_afun   : "\<lbrakk> \<Xi> f = (K', t, u)
+                   ; list_all2 (kinding K) ts K' 
+                   ; wellformed_fn (length K') t
+                   ; wellformed_fn (length K') u
+                   ; K \<turnstile> \<Gamma> consumed
+                   \<rbrakk> \<Longrightarrow> \<Xi>, K, \<Gamma> \<turnstile>2 AFun f ts : instantiate ts (TFun t u)"
+
+| typing_fun    : "\<lbrakk> \<Xi>, K', [Some t] \<turnstile>2 f : u 
+                   ; K \<turnstile> \<Gamma> consumed
+                   ; wellformed_fn (length K') t
+                   ; wellformed_fn (length K') u
+                   ; list_all2 (kinding K) ts K'
+                   \<rbrakk> \<Longrightarrow> \<Xi>, K, \<Gamma> \<turnstile>2 Fun f ts : instantiate ts (TFun t u)"
+
+| typing_app    : "\<lbrakk> K \<turnstile> \<Gamma> \<leadsto> \<Gamma>1 | \<Gamma>2
+                   ; \<Xi>, K, \<Gamma>1 \<turnstile>2 a : TFun x y
+                   ; \<Xi>, K, \<Gamma>2 \<turnstile>2 b : x
+                   \<rbrakk> \<Longrightarrow> \<Xi>, K, \<Gamma> \<turnstile>2 App a b : y"
+
+| typing_con    : "\<lbrakk> \<Xi>, K, \<Gamma> \<turnstile>2 x : t
+                   ; (tag,t) \<in> set ts
+                   ; distinct (map fst ts)
+                   ; list_all (wellformed_fn (length K) \<circ> snd) ts
+                   \<rbrakk> \<Longrightarrow> \<Xi>, K, \<Gamma> \<turnstile>2 Con ts tag x : TSum ts"
+
+| typing_prom   : "\<lbrakk> \<Xi>, K, \<Gamma> \<turnstile>2 x : TSum ts
+                   ; set ts \<subseteq> set ts'
+                   ; distinct (map fst ts')
+                   ; list_all (wellformed_fn (length K) \<circ> snd) ts'
+                   \<rbrakk> \<Longrightarrow> \<Xi>, K, \<Gamma> \<turnstile>2 Promote ts' x : TSum ts'"
+
+| typing_cast   : "\<lbrakk> \<Xi>, K, \<Gamma> \<turnstile>2 e : TPrim (Num \<tau>)
+                   ; upcast_valid \<tau> \<tau>' 
+                   \<rbrakk> \<Longrightarrow> \<Xi>, K, \<Gamma> \<turnstile>2 Cast \<tau>' e : TPrim (Num \<tau>')"
+
+| typing_tuple  : "\<lbrakk> K \<turnstile> \<Gamma> \<leadsto> \<Gamma>1 | \<Gamma>2
+                   ; \<Xi>, K, \<Gamma>1 \<turnstile>2 t : T 
+                   ; \<Xi>, K, \<Gamma>2 \<turnstile>2 u : U
+                   \<rbrakk> \<Longrightarrow> \<Xi>, K, \<Gamma> \<turnstile>2 Tuple t u : TProduct T U"
+
+| typing_split  : "\<lbrakk> K \<turnstile> \<Gamma> \<leadsto> \<Gamma>1 | \<Gamma>2
+                   ; \<Xi>, K, \<Gamma>1 \<turnstile>2 x : TProduct t u
+                   ; \<Xi>, K, (Some t)#(Some u)#\<Gamma>2 \<turnstile>2 y : t'
+                   \<rbrakk> \<Longrightarrow> \<Xi>, K, \<Gamma> \<turnstile>2 Split x y : t'" 
+
+| typing_let    : "\<lbrakk> K \<turnstile> \<Gamma> \<leadsto> \<Gamma>1 | \<Gamma>2 
+                   ; \<Xi>, K, \<Gamma>1 \<turnstile>2 x : t
+                   ; \<Xi>, K, (Some t # \<Gamma>2) \<turnstile>2 y : u
+                   \<rbrakk> \<Longrightarrow> \<Xi>, K, \<Gamma> \<turnstile>2 Let x y : u"
+
+| typing_letb   : "\<lbrakk> split_bang K is \<Gamma> \<Gamma>1 \<Gamma>2
+                   ; \<Xi>, K, \<Gamma>1 \<turnstile>2 x : t
+                   ; \<Xi>, K, (Some t # \<Gamma>2) \<turnstile>2 y : u
+                   ; E \<in> kinding_fn K t
+                   \<rbrakk> \<Longrightarrow> \<Xi>, K, \<Gamma> \<turnstile>2 LetBang is x y : u"
+
+| typing_case   : "\<lbrakk> K \<turnstile> \<Gamma> \<leadsto> \<Gamma>1 | \<Gamma>2
+                   ; \<Xi>, K, \<Gamma>1 \<turnstile>2 x : TSum ts
+                   ; (tag, t) \<in> set ts
+                   ; \<Xi>, K, (Some t # \<Gamma>2) \<turnstile>2 a : u
+                   ; \<Xi>, K, (Some (TSum (filter (\<lambda> x. fst x \<noteq> tag) ts)) # \<Gamma>2) \<turnstile>2 b : u
+                   \<rbrakk> \<Longrightarrow> \<Xi>, K, \<Gamma> \<turnstile>2 Case x tag a b : u" 
+
+| typing_esac   : "\<lbrakk> \<Xi>, K, \<Gamma> \<turnstile>2 x : TSum [(tag,t)]
+                   \<rbrakk> \<Longrightarrow> \<Xi>, K, \<Gamma> \<turnstile>2 Esac x : t"
+
+| typing_if     : "\<lbrakk> K \<turnstile> \<Gamma> \<leadsto> \<Gamma>1 | \<Gamma>2
+                   ; \<Xi>, K, \<Gamma>1 \<turnstile>2 x : TPrim Bool
+                   ; \<Xi>, K, \<Gamma>2 \<turnstile>2 a : t
+                   ; \<Xi>, K, \<Gamma>2 \<turnstile>2 b : t
+                   \<rbrakk> \<Longrightarrow> \<Xi>, K, \<Gamma> \<turnstile>2 If x a b : t"
+
+| typing_prim   : "\<lbrakk> \<Xi>, K, \<Gamma> \<turnstile>2* args : map TPrim ts 
+                   ; prim_op_type oper = (ts,t)
+                   \<rbrakk> \<Longrightarrow> \<Xi>, K, \<Gamma> \<turnstile>2 Prim oper args : TPrim t"
+
+| typing_lit    : "\<lbrakk> K \<turnstile> \<Gamma> consumed
+                   \<rbrakk> \<Longrightarrow> \<Xi>, K, \<Gamma> \<turnstile>2 Lit l : TPrim (lit_type l)" 
+
+| typing_unit   : "\<lbrakk> K \<turnstile> \<Gamma> consumed
+                   \<rbrakk> \<Longrightarrow> \<Xi>, K, \<Gamma> \<turnstile>2 Unit : TUnit"
+
+| typing_struct : "\<lbrakk> \<Xi>, K, \<Gamma> \<turnstile>2* es : ts
+                   ; ts' = zip ts (replicate (length ts) False)
+                   \<rbrakk> \<Longrightarrow> \<Xi>, K, \<Gamma> \<turnstile>2 Struct ts es : TRecord ts' Unboxed"
+
+| typing_member : "\<lbrakk> \<Xi>, K, \<Gamma> \<turnstile>2 e : TRecord ts s
+                   ; S \<in> kinding_fn K (TRecord ts s)
+                   ; f < length ts
+                   ; ts ! f = (t, False)
+                   \<rbrakk> \<Longrightarrow> \<Xi>, K, \<Gamma> \<turnstile>2 Member e f : t"
+
+| typing_take   : "\<lbrakk> K \<turnstile> \<Gamma> \<leadsto> \<Gamma>1 | \<Gamma>2 
+                   ; \<Xi>, K, \<Gamma>1 \<turnstile>2 e : TRecord ts s
+                   ; s \<noteq> ReadOnly
+                   ; f < length ts
+                   ; ts ! f = (t, False)
+                   ; S \<in> kinding_fn K t \<or> taken
+                   ; \<Xi>, K, (Some t # Some (TRecord (ts [f := (t,taken)]) s) # \<Gamma>2) \<turnstile>2 e' : u
+                   \<rbrakk> \<Longrightarrow> \<Xi>, K, \<Gamma> \<turnstile>2 Take e f e' : u"
+
+| typing_put    : "\<lbrakk> K \<turnstile> \<Gamma> \<leadsto> \<Gamma>1 | \<Gamma>2
+                   ; \<Xi>, K, \<Gamma>1 \<turnstile>2 e : TRecord ts s
+                   ; s \<noteq> ReadOnly
+                   ; f < length ts
+                   ; ts ! f = (t, taken)
+                   ; K \<turnstile> t :\<kappa> k
+                   ; D \<in> k \<or> taken
+                   ; \<Xi>, K, \<Gamma>2 \<turnstile>2 e' : t
+                   \<rbrakk> \<Longrightarrow> \<Xi>, K, \<Gamma> \<turnstile>2 Put e f e' : TRecord (ts [f := (t,False)]) s"
+
+| typing_all_empty : "\<Xi>, K, empty n \<turnstile>2* [] : []"
+
+| typing_all_cons  : "\<lbrakk> K \<turnstile> \<Gamma> \<leadsto> \<Gamma>1 | \<Gamma>2
+                      ; \<Xi>, K, \<Gamma>1 \<turnstile>2  e  : t
+                      ; \<Xi>, K, \<Gamma>2 \<turnstile>2* es : ts
+                      \<rbrakk> \<Longrightarrow> \<Xi>, K, \<Gamma> \<turnstile>2* (e # es) : (t # ts)"
+
+lemma typing2_and_ctx_wellformed_impl_wellformed:
+  assumes "ctx_wellformed_fn (length K) \<Gamma>"
+  shows
+    "\<Xi>, K, \<Gamma> \<turnstile>2 e : t \<Longrightarrow> wellformed_fn (length K) t"
+    "\<Xi>, K, \<Gamma> \<turnstile>2* es : ts \<Longrightarrow> list_all (wellformed_fn (length K)) ts"
+  using assms
+proof (induct rule: typing2_typing2_all.inducts)
+  case typing_var then show ?case
+    by (force dest: weakening_preservation simp add: Cogent.empty_def list_all_length ctx_wellformed_fn_def)
+next
+  case typing_afun then show ?case
+    by (auto intro!: wellformedfn_preserves_instantiate
+        simp add: kinding_iff_wellformedfn_and_kindingfn list_all2_conv_all_nth list_all_length)
+next
+  case typing_fun then show ?case
+    by (auto intro!: wellformedfn_preserves_instantiate
+        simp add: kinding_iff_wellformedfn_and_kindingfn list_all2_conv_all_nth list_all_length)
+next
+  case typing_letb then show ?case
+    by (force dest: split_bang_preserves_wellformed simp add: ctx_wellformed_fn_Cons)
+next
+  case (typing_case K \<Gamma> \<Gamma>1 \<Gamma>2 \<Xi> x ts tag t a u b)
+  moreover then have "wellformed_fn (length K) t"
+  proof -
+    have "list_all (\<lambda>x. wellformed_fn (length K) (snd x)) ts"
+      using typing_case
+      by (force dest: split_preserves_wellformed)
+    then show ?thesis
+      using typing_case
+      by (force simp add: list_all_iff)
+  qed
+  ultimately show ?case
+    by (force dest: split_preserves_wellformed simp add: ctx_wellformed_fn_Cons)
+next
+  case typing_struct then show ?case
+    by (simp add: list_all_length)
+next
+  case typing_member then show ?case
+    by (force simp add: list_all_length)
+next
+  case (typing_take K \<Gamma> \<Gamma>1 \<Gamma>2 \<Xi> e ts s f t taken e' u)
+  moreover have wellformed_t: "wellformed_fn (length K) t"
+    using typing_take
+    by (force dest: split_preserves_wellformed simp add: list_all_length)
+  moreover have "list_all (\<lambda>x. wellformed_fn (length K) (fst x)) (ts[f := (t, taken)])"
+  proof -
+    have "list_all (\<lambda>x. wellformed_fn (length K) (fst x)) ts"
+      using typing_take
+      by (force dest: split_preserves_wellformed simp add: list_all_length)
+    then show ?thesis
+      using typing_take wellformed_t
+      by (simp add: list_all_length nth_list_update)
+  qed
+  ultimately show ?case
+    by (force dest: split_preserves_wellformed simp add: ctx_wellformed_fn_Cons)
+next
+  case (typing_put K \<Gamma> \<Gamma>1 \<Gamma>2 \<Xi> e ts s f t taken k e')
+  moreover have "list_all (\<lambda>x. wellformed_fn (length K) (fst x)) ts"
+    using typing_put by (force dest: split_preserves_wellformed)
+  moreover have "wellformed_fn (length K) t"
+    using typing_put by (force dest: kinding_imp_wellformedfn)
+  ultimately show ?case
+    by (clarsimp simp add: list_all_length nth_list_update)
+qed (fastforce dest: split_preserves_wellformed simp add: ctx_wellformed_fn_Cons comp_def)+
+
+lemma typing2_imp_typing:
+  assumes "ctx_wellformed_fn (length K) \<Gamma>"
+  shows
+    "\<Xi>, K, \<Gamma> \<turnstile>2 e : t \<Longrightarrow> \<Xi>, K, \<Gamma> \<turnstile> e : t"
+    "\<Xi>, K, \<Gamma> \<turnstile>2* es : ts \<Longrightarrow> \<Xi>, K, \<Gamma> \<turnstile>* es : ts"
+  using assms
+proof (induct rule: typing2_typing2_all.inducts)
+  case typing_afun then show ?case
+    by (auto intro!: typing_typing_all.intros simp add: wellformed_iff_wellformedfn[simplified])
+next
+  case typing_fun then show ?case
+    by (auto
+        intro!: typing_typing_all.intros
+        simp add: wellformed_iff_wellformedfn[simplified] ctx_wellformed_fn_Cons
+        ctx_wellformed_fn_nil)
+next
+  case typing_con then show ?case
+    by (auto intro!: typing_typing_all.intros
+        simp add: wellformed_all_iff_wellformedfn_all[simplified] list.pred_map)
+next
+  case typing_prom then show ?case
+    by (auto intro!: typing_typing_all.intros
+        simp add: wellformed_all_iff_wellformedfn_all[simplified] list.pred_map)
+next
+  case (typing_split K \<Gamma> \<Gamma>1 \<Gamma>2 \<Xi> x t u y t')
+  moreover have
+    "wellformed_fn (length K) t"
+    "wellformed_fn (length K) u"
+    using typing_split
+    by (fastforce dest: typing2_and_ctx_wellformed_impl_wellformed split_preserves_wellformed)+
+  ultimately show ?case
+    by (auto intro!: typing_typing_all.intros dest: split_preserves_wellformed simp add: ctx_wellformed_fn_Cons)
+next
+  case typing_let then show ?case
+    by (auto intro!: typing_typing_all.intros simp add: ctx_wellformed_fn_Cons
+        dest: typing2_and_ctx_wellformed_impl_wellformed split_preserves_wellformed)
+next
+  case typing_letb then show ?case
+    by (fastforce intro!: typing_typing_all.intros
+        simp add: ctx_wellformed_fn_Cons kinding_iff_wellformedfn_and_kindingfn
+        dest: typing2_and_ctx_wellformed_impl_wellformed split_bang_preserves_wellformed)
+next
+  case (typing_case K \<Gamma> \<Gamma>1 \<Gamma>2 \<Xi> x ts tag t a u b)
+  moreover have wellformed_tsum: "wellformed_fn (length K) (TSum ts)"
+    using typing_case
+    by (blast dest: split_preserves_wellformed typing2_and_ctx_wellformed_impl_wellformed)
+  moreover have "wellformed_fn (length K) t"
+      using typing_case wellformed_tsum
+      by (force simp add: list_all_iff)
+  moreover have "distinct (map fst (filter (\<lambda>x. fst x \<noteq> tag) ts))"
+    using wellformed_tsum distinct_map_filter by force
+  moreover have "list_all (\<lambda>x. wellformed_fn (length K) (snd x)) (filter (\<lambda>x. fst x \<noteq> tag) ts)"
+    using wellformed_tsum
+    by (force intro: list_all_imp_list_all_filtered)
+  ultimately show ?case
+    by (auto intro!: typing_typing_all.intros dest: split_preserves_wellformed
+        simp add: ctx_wellformed_fn_Cons)
+next
+  case (typing_member \<Xi> K \<Gamma> e ts s f t)
+  then show ?case
+  proof (intro typing_typing_all.intros)
+    show "K \<turnstile> TRecord ts s :\<kappa> kinding_fn K (TRecord ts s)"
+      using typing_member
+      by (force dest: typing2_and_ctx_wellformed_impl_wellformed
+          simp add: wellformedfn_and_kindingfn_imp_kinding)
+  qed auto
+next
+  case (typing_take K \<Gamma> \<Gamma>1 \<Gamma>2 \<Xi> e ts s f t taken e' u)
+  moreover have wellformed_rec: "wellformed_fn (length K) (TRecord ts s)"
+    using typing_take
+    by (blast dest: split_preserves_wellformed typing2_and_ctx_wellformed_impl_wellformed)
+  moreover have wellformed_t: "wellformed_fn (length K) t"
+    using wellformed_rec typing_take.hyps
+    by (force simp add: list_all_length)
+  moreover then have "ctx_wellformed_fn (length K) (Some t # Some (TRecord (ts[f := (t, taken)]) s) # \<Gamma>2)"
+    using wellformed_t typing_take wellformed_rec wellformed_t
+    by (auto dest: split_preserves_wellformed simp add: list_all_update_weak ctx_wellformed_fn_Cons)
+  ultimately show ?case
+  proof (intro typing_typing_all.intros)
+    show "K \<turnstile> t :\<kappa> kinding_fn K t"
+      using typing_member wellformed_t
+      by (force simp add: wellformedfn_and_kindingfn_imp_kinding)
+  qed (auto dest: split_preserves_wellformed)
+qed (blast intro!: typing_typing_all.intros dest: split_preserves_wellformed)+
+
+end
